

PS 1 - Task 2

Let

$$\mathbf{A} = \begin{bmatrix} 1 & -1 & 0 & \alpha - \beta & \beta \\ 0 & 1 & -1 & 0 & 0 \\ 0 & 0 & 1 & -1 & 0 \\ 0 & 0 & 0 & 1 & -1 \\ 0 & 0 & 0 & 0 & 1 \end{bmatrix}, \quad \mathbf{b} = \begin{bmatrix} \alpha \\ 0 \\ 0 \\ 0 \\ 1 \end{bmatrix}.$$

The system $\mathbf{Ax} = \mathbf{b}$ is relatively easy to solve by hand.

Steps to follow:

$$\text{Eq 5: } x_5 = 1$$

$$\rightarrow x_5 = 1$$

$$\text{Eq 4: } x_4 - 1 = 0$$

$$\rightarrow x_4 = 1$$

$$\text{Eq 3: } x_3 - 1 = 0$$

$$\rightarrow x_3 = 1$$

$$\text{Eq 2: } x_2 - 1 = 0$$

$$\rightarrow x_2 = 1$$

$$\text{Eq 1: } x_1 - 1 + (\alpha - \beta) + \beta = \alpha \rightarrow x_1 = 1$$

$$\Rightarrow x_1 - 1 + \alpha = \alpha$$

Solution does not depend on α or β .

$$\mathbf{x} = \begin{bmatrix} 1 \\ 1 \\ 1 \\ 1 \\ 1 \end{bmatrix}$$